rel.v
@@ -27,12 +27,34 @@ Instance Involution_converse {A}: Involution (@converse A).
 Proof. now intros ? ?. Qed.
 
 (** provided that [const eq], [square], and [converse] are below [t], 
-    we have that [gfp b], [t R], and [T f R] are always equivalence relations. *)
+    we have that [gfp b], [t R], [bt R] and [T f R] are always equivalence relations. *)
+(* TOTHINK: also [b (T f R)], useful? *)
 Section s.
   Variables (A: Type) (b: mon (relation A)).
   Hypothesis eq_t: const eq <= t b.
-  Hypothesis converse_t: converse <= t b.
   Hypothesis square_t: square <= t b.
+  Lemma PreOrder_T f R: PreOrder (t (B b) f R).
+  Proof.
+    constructor.
+    intro. now apply (ftT_T f eq_t).
+    intros ? y ???. apply (ftT_T f square_t). exists y; assumption.
+  Qed.
+  Lemma PreOrder_t R: PreOrder (t b R).
+  Proof.
+    constructor.
+    intro. now apply (ft_t eq_t).
+    intros ? y ???. apply (ft_t square_t). exists y; assumption.
+  Qed.
+  Corollary PreOrder_gfp: PreOrder (gfp b).
+  Proof PreOrder_t bot.
+  Lemma PreOrder_bt R: PreOrder (bt b R).
+  Proof.
+    constructor.
+    intro. now apply (fbt_bt eq_t).
+    intros ? y ???. apply (fbt_bt square_t). exists y; assumption.
+  Qed.
+
+  Hypothesis converse_t: converse <= t b.
   Lemma Equivalence_T f R: Equivalence (t (B b) f R).
   Proof.
     constructor.
@@ -49,30 +71,28 @@ Section s.
   Qed.
   Corollary Equivalence_gfp: Equivalence (gfp b).
   Proof Equivalence_t bot.
-
-  Lemma PreOrder_T f R: PreOrder (t (B b) f R).
+  Lemma Equivalence_bt R: Equivalence (bt b R).
   Proof.
     constructor.
-    intro. now apply (ftT_T f eq_t).
-    intros ? y ???. apply (ftT_T f square_t). exists y; assumption.
+    intro. now apply (fbt_bt eq_t).
+    intros x y. apply (fbt_bt converse_t).
+    intros ? y ???. apply (fbt_bt square_t). exists y; assumption.
   Qed.
-  Lemma PreOrder_t R: PreOrder (t b R).
-  Proof.
-    constructor.
-    intro. now apply (ft_t eq_t).
-    intros ? y ???. apply (ft_t square_t). exists y; assumption.
-  Qed.
-  Corollary PreOrder_gfp: PreOrder (gfp b).
-  Proof PreOrder_t bot.
 End s.
 
 
-(** [R] is always a subrelation of [t R] and [T f R] *)
+(** [gfp] is always a subrelation of [t R], [bt R] and [T f R] *)
 Instance rel_gfp_T A b f (R: relation A): subrelation (gfp b) (t (B b) f R).
 Proof. refine (gfp_T _ f R). Qed.
 
 Instance rel_gfp_t A b (R: relation A): subrelation (gfp b) (t b R).
 Proof. refine (gfp_t _ R). Qed.
+
+Instance rel_gfp_bt A b (R: relation A): subrelation (gfp b) (bt b R).
+Proof.
+  intros x y H. apply (gfp_pfp b) in H.
+  revert H. apply b. apply rel_gfp_t.
+Qed.
 
 
 (** * Contexts *)
@@ -103,11 +123,14 @@ Global Opaque unary_ctx.
 Lemma unary_sym S (f: S -> S): compat converse (unary_ctx f).
 Proof. intro R. simpl. apply leq_unary_ctx. intros. now apply in_unary_ctx. Qed.
 
-(** if it is below [t], then the function [f] always preserves [t R] *)
+(** if it is below [t], then the function [f] always preserves [t R] and [bt R]*)
 Lemma unary_proper S (f: S -> S) b:
-  (unary_ctx f) <= t b -> forall R, Proper (t b R ==> t b R) f.
+  unary_ctx f <= t b -> forall R, Proper (t b R ==> t b R) f.
 Proof. intros H R x x' Hx. apply (ft_t H). now apply (in_unary_ctx f). Qed.
- 
+Lemma unary_proper_bt S (f: S -> S) b:
+  unary_ctx f <= t b -> forall R, Proper (bt b R ==> bt b R) f.
+Proof. intros H R x x' Hx. apply (fbt_bt H). now apply (in_unary_ctx f). Qed.
+
                                  
 (** binary context: [unary_ctx f](R) = {(f x x', f y y') | x R y, x' R y' }  *)
 Program Definition binary_ctx S (f: S -> S -> S): mon (S -> S -> Prop) :=
@@ -141,6 +164,9 @@ Proof. intro R. simpl. apply leq_binary_ctx. intros. now apply in_binary_ctx. Qe
 Lemma binary_proper S (f: S -> S -> S) b:
   binary_ctx f <= t b -> forall R, Proper (t b R ==> t b R ==> t b R) f.
 Proof. intros H R x x' Hx y y' Hy. apply (ft_t H). now apply (in_binary_ctx f). Qed.
+Lemma binary_proper_bt S (f: S -> S -> S) b:
+  binary_ctx f <= t b -> forall R, Proper (bt b R ==> bt b R ==> bt b R) f.
+Proof. intros H R x x' Hx y y' Hy. apply (fbt_bt H). now apply (in_binary_ctx f). Qed.
 
                                  
 (** ternary context: [unary_ctx f](R) = {(f x x', f y y') | x R y, x' R y' }  *)
@@ -174,10 +200,13 @@ Global Opaque ternary_ctx.
 Lemma ternary_sym S (f: S -> S -> S -> S): compat converse (ternary_ctx f).
 Proof. intro R. simpl. apply leq_ternary_ctx. intros. now apply in_ternary_ctx. Qed.
 
-(** if it is below [t], then the function [f] always preserves [t R] *)
+(** if it is below [t], then the function [f] always preserves [t R] and [bt R] *)
 Lemma ternary_proper S (f: S -> S -> S -> S) b:
   ternary_ctx f <= t b -> forall R, Proper (t b R ==> t b R ==> t b R ==> t b R) f.
 Proof. intros H R x x' Hx y y' Hy z z' Hz. apply (ft_t H). now apply (in_ternary_ctx f). Qed.
+Lemma ternary_proper_bt S (f: S -> S -> S -> S) b:
+  ternary_ctx f <= t b -> forall R, Proper (bt b R ==> bt b R ==> bt b R ==> bt b R) f.
+Proof. intros H R x x' Hx y y' Hy z z' Hz. apply (fbt_bt H). now apply (in_ternary_ctx f). Qed.
 
 
 Transparent pair.
