tests.v
@@ -8,7 +8,7 @@ Section s.
   Infix "~" := (gfp b) (at level 80).
   Notation "x ≡[ R ] y" := (t b R x y) (at level 80). 
   Notation "x ≡ y" := (t b _ x y) (at level 80). 
-  Notation "x [≡] y" := (b (body (t b) _) x y) (at level 80).
+  Notation "x [≡] y" := (bt b _ x y) (at level 80).
   Goal 5 ~ 6.
     coinduction R H.
     Restart.
